size_t simplification

specs/Spec.Poly1305.fst
@@ -1,14 +1,10 @@
 module Spec.Poly1305
 
-module ST = FStar.HyperStack.ST
-
-open FStar.Math.Lib
 open FStar.Mul
-open FStar.Seq
-open FStar.UInt8
-open FStar.Endianness
+open Spec.Lib.IntTypes
+open Spec.Lib.IntSeq
 open Spec.Poly1305.Lemmas
-#set-options "--initial_fuel 0 --max_fuel 0 --initial_ifuel 0 --max_ifuel 0"
+#set-options "--z3rlimit 30 --initial_fuel 0 --max_fuel 0 --initial_ifuel 0 --max_ifuel 0"
 
 (* Field types and parameters *)
 let prime =  pow2 130 - 5
@@ -19,45 +15,48 @@ let zero : elem = 0
 let one  : elem = 1
 let op_Plus_At = fadd
 let op_Star_At = fmul
-(* Type aliases *)
-let op_Amp_Bar = UInt.logand #128
-type word = w:bytes{length w <= 16}
-type word_16 = w:bytes{length w = 16}
-type tag = word_16
-type key = lbytes 32
-type text = seq word
+
+
+type lbytes (s:size_t) = intseq U8 s
+let nat_from_bytes_le = nat_from_intseq_le
+
+let blocksize : size_t = 16
+let keysize   : size_t = 32
+
+type block = lbytes blocksize
+type tag   = lbytes blocksize
+type key   = lbytes keysize
 
 (* Specification code *)
-let encode (w:word) =
-  (pow2 (8 * length w)) `fadd` (little_endian w)
+let encode_block (w:block) =
+  pow2 128 `fadd` nat_from_bytes_le  w 
 
-let rec poly (txt:text) (r:e:elem) : Tot elem (decreases (length txt)) =
-  if length txt = 0 then zero
-  else
-    let a = poly (Seq.tail txt) r in
-    let n = encode (Seq.head txt) in
-    (n `fadd` a) `fmul` r
+let encode_last (#l:size_t{l < blocksize}) (w:lbytes l) =
+  assert (pow2 (8 * l) < pow2 128);
+  pow2 (8 * l) `fadd` nat_from_bytes_le w
 
-let encode_r (rb:word_16) =
-  (little_endian rb) &| 0x0ffffffc0ffffffc0ffffffc0fffffff
+val poly: #len:size_t -> txt:lbytes len -> r:elem -> acc:elem
+let poly #len txt r =
+  let blocks = len / blocksize in
+  let rem = len % blocksize in
+  repeati blocks
+    (fun i acc -> 
+      let b = sub txt (i * blocksize) blocksize in
+      let n = encode_block b in
+      (n `fadd` acc) `fmul` r) 0
+  
+let encode_r (rb:block) : elem =
+    uint_to_nat ((uint_from_bytes_le #U128 rb) &. 
+		  u128 0x0ffffffc0ffffffc0ffffffc0fffffff)
 
-let finish (a:elem) (s:word_16) : Tot tag =
-  let n = (a + little_endian s) % pow2 128 in
-  little_bytes 16ul n
+let finish (a:elem) (s:block) : Tot tag =
+  let n = (a + nat_from_bytes_le s) % pow2 128 in
+  nat_to_bytes_le 16 n
 
-let append_last = snoc
-
-let rec encode_bytes (txt:bytes) : Tot text (decreases (length txt)) =
-  if length txt = 0 then createEmpty
-  else
-    let w, txt = split txt (min (length txt) 16) in
-    append_last (encode_bytes txt) w
-
-let poly1305 (msg:bytes) (k:key) : Tot tag =
-  let text = encode_bytes msg in
-  let r = encode_r (slice k 0 16) in
-  let s = slice k 16 32 in
-  finish (poly text r) s
+let poly1305 (#len:size_t) (msg:lbytes len) (k:key) : Tot tag =
+  let r = encode_r (sub k 0 16) in
+  let s = sub k 16 16 in
+  finish (poly msg r) s
 
 
 (* ********************* *)
@@ -66,28 +65,29 @@ let poly1305 (msg:bytes) (k:key) : Tot tag =
 
 #reset-options "--initial_fuel 0 --max_fuel 0 --z3rlimit 20"
 
-unfold let msg = [
+let msg = List.Tot.map u8uy [
   0x43uy; 0x72uy; 0x79uy; 0x70uy; 0x74uy; 0x6fuy; 0x67uy; 0x72uy;
   0x61uy; 0x70uy; 0x68uy; 0x69uy; 0x63uy; 0x20uy; 0x46uy; 0x6fuy;
   0x72uy; 0x75uy; 0x6duy; 0x20uy; 0x52uy; 0x65uy; 0x73uy; 0x65uy;
   0x61uy; 0x72uy; 0x63uy; 0x68uy; 0x20uy; 0x47uy; 0x72uy; 0x6fuy;
-  0x75uy; 0x70uy ]
+  0x75uy; 0x70uy]
 
-unfold let k = [
+let k = List.Tot.map u8uy [
   0x85uy; 0xd6uy; 0xbeuy; 0x78uy; 0x57uy; 0x55uy; 0x6duy; 0x33uy;
   0x7fuy; 0x44uy; 0x52uy; 0xfeuy; 0x42uy; 0xd5uy; 0x06uy; 0xa8uy;
   0x01uy; 0x03uy; 0x80uy; 0x8auy; 0xfbuy; 0x0duy; 0xb2uy; 0xfduy;
-  0x4auy; 0xbfuy; 0xf6uy; 0xafuy; 0x41uy; 0x49uy; 0xf5uy; 0x1buy ]
+  0x4auy; 0xbfuy; 0xf6uy; 0xafuy; 0x41uy; 0x49uy; 0xf5uy; 0x1buy]
 
-unfold let expected = [
+let expected = List.Tot.map u8uy [
   0xa8uy; 0x06uy; 0x1duy; 0xc1uy; 0x30uy; 0x51uy; 0x36uy; 0xc6uy;
-  0xc2uy; 0x2buy; 0x8buy; 0xafuy; 0x0cuy; 0x01uy; 0x27uy; 0xa9uy ]
+  0xc2uy; 0x2buy; 0x8buy; 0xafuy; 0x0cuy; 0x01uy; 0x27uy; 0xa9uy]
 
 let test () : Tot bool =
   assert_norm(List.Tot.length msg      = 34);
   assert_norm(List.Tot.length k        = 32);
   assert_norm(List.Tot.length expected = 16);
-  let msg      = createL msg in
-  let k        = createL k   in
-  let expected = createL expected in
-  poly1305 msg k = expected
+  let msg      : lseq uint8 34  = createL #uint8 msg in
+  let k        : lseq uint8 keysize  = createL #uint8 k   in
+  let expected : lseq uint8 blocksize = createL #uint8 expected in
+  let mac      : lseq uint8 blocksize = poly1305 msg k in
+  for_all2 #uint8 #uint8 (fun a b -> uint_to_nat a = uint_to_nat b) mac expected
