specs/lib/Spec.Lib.IntSeq.fst
@@ -5,11 +5,11 @@ open Spec.Lib.IntTypes
 
 #set-options "--z3rlimit 100"
 
-type lseq (a:Type0) (len:size_t) = s:list a {List.Tot.length s = size_to_nat len}
+let lseq (a:Type0) (len:size_t) =  s:list a {List.Tot.length s = len}
 
-val create_: #a:Type -> len:size_t -> init:a -> Tot (lseq a len) (decreases (size_to_nat len))
+val create_: #a:Type -> len:size_t -> init:a -> Tot (lseq a len) (decreases (len))
 let rec create_ #a len x = 
-  if size_to_nat len = 0 then []
+  if len = 0 then []
   else
     let t = create_ #a (size_decr len) x in
     x :: t 
@@ -18,35 +18,35 @@ let create = create_
 let createL #a l = l
 
 
-val repeat_: #a:Type -> n:size_t -> (a -> Tot a) -> a -> Tot (a) (decreases (size_to_nat n))
+val repeat_: #a:Type -> n:size_t -> (a -> Tot a) -> a -> Tot (a) (decreases (n))
 let rec repeat_ #a n f x = 
-  match size_to_nat n with
+  match n with
   | 0 -> x
   | _ -> repeat_ #a (size_decr n) f (f x)
 let repeat = repeat_
 
-val repeati_: #a:Type -> i:size_t -> n:size_t{size_to_nat i <= size_to_nat n} -> (size_t -> a -> Tot a) -> a -> Tot (a) (decreases (size_to_nat n - size_to_nat i))
+val repeati_: #a:Type -> i:size_t -> n:size_t{i <= n} -> (s:size_t{s < n} -> a -> Tot a) -> a -> Tot (a) (decreases (n - i))
 let rec repeati_ #a i n f x = 
-  if size_to_nat i = size_to_nat n then x
+  if i = n then x
   else repeati_ #a (size_incr i) n f (f i x)
-let repeati #a = repeati_ #a (nat_to_size 0)
+let repeati #a = repeati_ #a ( 0)
 
-val fold_left_: #a:Type -> #b:Type -> #len:size_t -> (a -> b -> Tot b) -> lseq a len -> b -> Tot (b) (decreases (size_to_nat len))
+val fold_left_: #a:Type -> #b:Type -> #len:size_t -> (a -> b -> Tot b) -> lseq a len -> b -> Tot (b) (decreases (len))
 let rec fold_left_ #a #b #len f l init =
   match l with
   | [] -> init 
   | h :: t -> fold_left_ #a #b #(size_decr len) f t (f h init)
 let fold_left = fold_left_
 
-val fold_lefti_: #a:Type -> #b:Type -> #fulllen:size_t -> #len:size_t{size_to_nat len <= size_to_nat fulllen} -> (size_t -> a -> b -> Tot b) -> lseq a len -> b -> Tot (b) (decreases (size_to_nat len))
+val fold_lefti_: #a:Type -> #b:Type -> #fulllen:size_t -> #len:size_t{len <= fulllen} -> (size_t -> a -> b -> Tot b) -> lseq a len -> b -> Tot (b) (decreases (len))
 let rec fold_lefti_ #a #b #fulllen #len f l init =
   match l with
   | [] -> init 
-  | h :: t -> let i = size_sub fulllen len in 
+  | h :: t -> let i = fulllen - len in 
 	    fold_lefti_ #a #b #fulllen #(size_decr len) f t (f i h init)
 let fold_lefti #a #b #len = fold_lefti_ #a #b #len #len
 
-val map_: #a:Type -> #b:Type -> #len:size_t -> (a -> Tot b) -> lseq a len -> Tot (lseq b len) (decreases (size_to_nat len))
+val map_: #a:Type -> #b:Type -> #len:size_t -> (a -> Tot b) -> lseq a len -> Tot (lseq b len) (decreases (len))
 let rec map_ #a #b #len f x =
   match x with
   | [] -> []
@@ -57,7 +57,17 @@ let rec map_ #a #b #len f x =
 let map = map_
 
 
-val ghost_map_: #a:Type -> #b:Type -> #len:size_t -> (a -> GTot b) -> lseq a len -> GTot (lseq b len) (decreases (size_to_nat len))
+val for_all_: #a:Type -> #len:size_t -> (a -> Tot bool) -> lseq a len -> Tot bool (decreases (len))
+let rec for_all_ #a #len f x =
+  match x with
+  | [] -> true
+  | h :: t -> 
+	 let t' : lseq a (size_decr len) = t in
+	 f h && for_all_ #a #(size_decr len) f t'
+
+let for_all = for_all_
+
+val ghost_map_: #a:Type -> #b:Type -> #len:size_t -> (a -> GTot b) -> lseq a len -> GTot (lseq b len) (decreases (len))
 let rec ghost_map_ #a #b #len f x = match x with
   | [] -> []
   | h :: t -> 
@@ -66,7 +76,7 @@ let rec ghost_map_ #a #b #len f x = match x with
 
 let ghost_map = ghost_map_
 
-val map2_: #a:Type -> #b:Type -> #c:Type -> #len:size_t -> (a -> b -> Tot c) -> lseq a len -> lseq b len -> Tot (lseq c len) (decreases (size_to_nat len))
+val map2_: #a:Type -> #b:Type -> #c:Type -> #len:size_t -> (a -> b -> Tot c) -> lseq a len -> lseq b len -> Tot (lseq c len) (decreases (len))
 let rec map2_ #a #b #c #len f x y = match x,y with
   | [],[] -> []
   | h1 :: t1, h2 :: t2 -> 
@@ -76,98 +86,111 @@ let rec map2_ #a #b #c #len f x y = match x,y with
 
 let map2 = map2_
 
-val index_: #a:Type -> #len:size_t{size_to_nat len > 0} -> lseq a len -> n:size_t{size_to_nat n < size_to_nat len} -> Tot a (decreases (size_to_nat n))
+val for_all2_: #a:Type -> #b:Type -> #len:size_t -> (a -> b -> Tot bool) -> lseq a len -> lseq b len -> Tot (bool) (decreases (len))
+let rec for_all2_ #a #b #len f x y = match x,y with
+  | [],[] -> true
+  | h1 :: t1, h2 :: t2 -> 
+	 let t1' : lseq a (size_decr len) = t1 in
+	 let t2' : lseq b (size_decr len) = t2 in
+	 f h1 h2 && for_all2_ #a #b #(size_decr len) f t1' t2'
+
+let for_all2 = for_all2_
+
+val index_: #a:Type -> #len:size_t{len > 0} -> lseq a len -> n:size_t{n < len} -> Tot a (decreases (n))
 let rec index_ #a #len l i = 
-  match size_to_nat i, l with
+  match i, l with
   | 0, h::t -> h
   | n, h::t -> index_ #a #(size_decr len) t (size_decr i)
 
 let index = index_
 
-val upd_: #a:Type -> #len:size_t -> lseq a len -> n:size_t{size_to_nat n < size_to_nat len /\ size_to_nat len > 0} -> x:a -> Tot (lseq a len) (decreases (size_to_nat n))
+val upd_: #a:Type -> #len:size_t -> lseq a len -> n:size_t{n < len /\ len > 0} -> x:a -> Tot (lseq a len) (decreases (n))
 let rec upd_ #a #len l i x = 
-  match size_to_nat i,l with
+  match i,l with
   | 0, h::t -> x::t
   | n, h::t -> h::upd_ #a #(size_decr len) t (size_decr i) x
 
 let upd = upd_
 
-val prefix_: #a:Type -> #len:size_t -> lseq a len -> n:size_t{size_to_nat n <= size_to_nat len} -> Tot (lseq a n) (decreases (size_to_nat n))
+val prefix_: #a:Type -> #len:size_t -> lseq a len -> n:size_t{n <= len} -> Tot (lseq a n) (decreases (n))
 let rec prefix_ #a #len l n =
-  match size_to_nat n,l with
+  match n,l with
   | 0, _ -> []
   | n', h::t -> h::prefix_ #a #(size_decr len) t (size_decr n)
 
 let prefix = prefix_
 
-val suffix_: #a:Type -> #len:size_t -> lseq a len -> n:size_t{size_to_nat n <= size_to_nat len} -> fin:size_t{fin = size_sub len n} -> Tot (lseq a fin) (decreases (size_to_nat n))
+val suffix: #a:Type -> #len:size_t -> lseq a len -> n:size_t{n <= len} -> Tot (lseq a (len - n)) (decreases (n))
+let rec suffix #a #len l n =
+  match n,l with
+  | 0, _ ->   l
+  | _, h::t -> suffix #a #(size_decr len) t (size_decr n) 
 
-let rec suffix_ #a #len l n fin =
-  match size_to_nat n,l with
-  | 0, _ ->  
-    assert (fin = len);
-    l
-  | _, h::t -> 
-    assert(fin = size_sub (size_decr len) (size_decr n));
-    suffix_ #a #(size_decr len) t (size_decr n) fin
-
-
-let suffix #a #len l n = suffix_ #a #len l n (size_sub len n)
-
-let rec slice #a #len l s n = 
+let sub #a #len l s n = 
   let suf = suffix #a #len l s in
-  prefix #(size_sub len s) suf n
+  prefix #(len - s) suf n
 
-val last: #a:Type -> #len:size_t{size_to_nat len > 0} -> x:lseq a len -> a
+let slice #a #len l s f = sub #a #len l s (f-s)
+
+val last: #a:Type -> #len:size_t{len > 0} -> x:lseq a len -> a
 let last #a #len x = index #a #len x (size_decr len)
 
-val snoc: #a:Type -> #len:size_t{size_to_nat len < maxint U32} -> i:lseq a len -> x:a -> Tot (o:lseq a (size_incr len){i == prefix #(size_incr len) o len /\ last o == x}) (decreases (size_to_nat len))
+val snoc: #a:Type -> #len:size_t{len < maxint U32} -> i:lseq a len -> x:a -> Tot (o:lseq a (size_incr len){i == prefix #(size_incr len) o len /\ last o == x}) (decreases (len))
 let rec snoc #a #len i x = 
   match i with 
   | [] -> [x] 
   | h::t -> h::snoc #a #(size_decr len) t x
 
-val update_prefix: #a:Type -> #len:size_t -> lseq a len -> n:size_t{size_to_nat n <= size_to_nat len} -> lseq a n -> Tot (lseq a len) (decreases (size_to_nat len))
+val update_prefix: #a:Type -> #len:size_t -> lseq a len -> n:size_t{n <= len} -> lseq a n -> Tot (lseq a len) (decreases (len))
 let rec update_prefix #a #len l n l' =
-  match size_to_nat n,l,l' with
+  match n,l,l' with
   | 0, _, _ -> l
   | _, h::t, h'::t' -> h':: update_prefix #a #(size_decr len) t (size_decr n) t'
 
-val update_slice_: #a:Type -> #len:size_t -> lseq a len -> start:size_t -> n:size_t{size_to_nat start + size_to_nat n <= size_to_nat len} -> lseq a n -> Tot (lseq a len) (decreases (size_to_nat len))
-let rec update_slice_ #a #len l s n l' = 
-  match size_to_nat s,l with 
+val update_sub_: #a:Type -> #len:size_t -> lseq a len -> start:size_t -> n:size_t{start + n <= len} -> lseq a n -> Tot (lseq a len) (decreases (len))
+let rec update_sub_ #a #len l s n l' = 
+  match s,l with 
   | 0, l -> update_prefix #a #len l n l'
-  | _, h::t -> h:: update_slice_ #a #(size_decr len) t (size_decr s) n l'
+  | _, h::t -> h:: update_sub_ #a #(size_decr len) t (size_decr s) n l'
 
-let update_slice = update_slice_ 
+let update_sub = update_sub_ 
 
-val nat_from_intseq_be:#t:inttype -> #len:size_t -> b:intseq t len -> Tot nat (decreases (size_to_nat len))
-let rec nat_from_intseq_be #t #len b = 
-  if size_to_nat len = 0 then 0
+let update_slice #a #len l s f sl = update_sub #a #len l s (f-s) sl
+
+val nat_from_intseq_be_:#t:inttype -> #len:size_t -> b:intseq t len -> Tot (n:nat{n < pow2 (len * bits t)})  (decreases (len))
+let rec nat_from_intseq_be_ #t #len b = 
+  if len = 0 then 0
   else
     let l = uint_to_nat #t (last #(uint_t t) #len b) in
     let pre : intseq t (size_decr len) = prefix #len b (size_decr len) in
-    l + (pow2 (bits t)) * (nat_from_intseq_be #t #(size_decr len) pre)
+    admit();
+    l + (pow2 (bits t)) * (nat_from_intseq_be_ #t #(size_decr len) pre)
 
-val nat_from_intseq_le:#t:inttype -> #len:size_t -> b:intseq t len -> Tot nat (decreases (size_to_nat len))
-let rec nat_from_intseq_le #t #len (b:intseq t len)  =
-  match size_to_nat len,b with
+let nat_from_intseq_be = nat_from_intseq_be_
+
+
+val nat_from_intseq_le_:#t:inttype -> #len:size_t -> b:intseq t len -> Tot (n:nat{n < pow2 (len * bits t)}) (decreases (len))
+let rec nat_from_intseq_le_ #t #len (b:intseq t len)  =
+  match len,b with
   | 0, _ -> (0) 
   | _, h::tt -> 
-    uint_to_nat h + pow2 (bits t) * (nat_from_intseq_le #t #(size_decr len) tt)
+    admit();
+    uint_to_nat h + pow2 (bits t) * (nat_from_intseq_le_ #t #(size_decr len) tt)
+
+let nat_from_intseq_le = nat_from_intseq_le_
 
 val nat_to_bytes_be: 
-  len:size_t -> n:nat{ n < pow2 (8 * size_to_nat len)} ->
-  Tot (b:intseq U8 len {n == nat_from_intseq_be #U8 #len b}) (decreases (size_to_nat len))
+  len:size_t -> n:nat{ n < pow2 (8 * len)} ->
+  Tot (b:intseq U8 len {n == nat_from_intseq_be #U8 #len b}) (decreases (len))
 #reset-options "--z3rlimit 200"
 let rec nat_to_bytes_be len n = 
-  if size_to_nat len = 0 then [] 
+  if len = 0 then [] 
   else (
     let len' = size_decr len in 
     let byte = u8 (n % 256) in
     let n' =  n / 256 in 
-    Math.Lemmas.pow2_plus 8 (8 * size_to_nat len');
-    assume( n' < pow2 (8 * size_to_nat len' ));
+    Math.Lemmas.pow2_plus 8 (8 * len');
+    assume( n' < pow2 (8 * len' ));
     let b' : intseq U8 len' = nat_to_bytes_be len' n' in
     let b  : intseq U8 len = snoc #uint8 #len' b' byte in
     assert(b' == prefix b len');
@@ -175,35 +198,37 @@ let rec nat_to_bytes_be len n =
     admit();
     b)
 
-val nat_to_bytes_le:
-  len:size_t -> n:nat{n < pow2 (8 * size_to_nat len)} ->
-  Tot (b:intseq U8 len {n == nat_from_intseq_le #U8 #len b}) (decreases (size_to_nat len))
-let rec nat_to_bytes_le len n = 
-  if size_to_nat len = 0 then  []
+val nat_to_bytes_le_:
+  len:size_t -> n:nat{n < pow2 (8 * len)} ->
+  Tot (b:intseq U8 len {n == nat_from_intseq_le #U8 #len b}) (decreases (len))
+let rec nat_to_bytes_le_ len n = 
+  if len = 0 then  []
   else
     let len = size_decr len in 
     let byte = u8 (n % 256) in
     let n' = n / 256 in 
-    Math.Lemmas.pow2_plus 8 (8 * size_to_nat len);
-    assert(n' < pow2 (8 * size_to_nat len ));
-    let b' : intseq U8 len = nat_to_bytes_le len n' in
+    Math.Lemmas.pow2_plus 8 (8 * len);
+    assert(n' < pow2 (8 * len ));
+    let b' : intseq U8 len = nat_to_bytes_le_ len n' in
     let b = byte :: b' in
     admit();
     b
 
+let nat_to_bytes_le = nat_to_bytes_le_
+
 let uint_to_bytes_le #t n = 
   admit();
-  nat_to_bytes_le (nat_to_size (numbytes t)) (uint_to_nat n)
+  nat_to_bytes_le (numbytes t) (uint_to_nat n)
 let uint_to_bytes_be #t n = 
   admit();
-  nat_to_bytes_be (nat_to_size (numbytes t)) (uint_to_nat n)
+  nat_to_bytes_be (numbytes t) (uint_to_nat n)
 let uint_from_bytes_le #t b = 
-  let n = nat_from_intseq_le #U8 #(nat_to_size (numbytes t)) b in
+  let n = nat_from_intseq_le #U8 #(numbytes t) b in
   admit();
   nat_to_uint #t n
   
 let uint_from_bytes_be #t b = 
-  let n = nat_from_intseq_be #U8 #(nat_to_size (numbytes t)) b in
+  let n = nat_from_intseq_be #U8 #(numbytes t) b in
   admit();
   nat_to_uint #t n
 
